Test/dafny0/StatementExpressions.dfy
@@ -1,0 +1,58 @@
+ghost method M(n: nat) //returns (y: nat)
+{
+  var y := F(n, 0);
+}
+function F(n: nat, p: int): nat
+{
+  calc {
+    100;
+  <  { if n != 0 { M(n-1); } }
+    102;
+  }
+  n
+}
+
+ghost method MM(n: nat) returns (y: nat)
+  decreases n, 0;
+{
+  if n != 0 {
+    y := FF(n-1);
+  }
+}
+function FF(n: nat): nat
+  decreases n, 1;
+{
+  calc {
+    100;
+  <  { var y := MM(n); }
+    102;
+  }
+  n
+}
+
+ghost method P(n: nat)
+{
+  if n != 0 {
+    var y :=
+      calc {
+        12;
+        { P(n-1); }
+        12;
+      }
+      100;
+    assert y == 100;
+  }
+}
+ghost method Q(n: nat)
+{
+  if n != 0 {
+    var y :=
+      calc {
+        12;
+        { Q(n+1); }  // error: cannot prove termination
+        12;
+      }
+      100;
+    assert y == 102;  // error: assertion does not hold
+  }
+}
